tree typechecks

tla-tree/CrashSafeTree.dfy
@@ -23,6 +23,12 @@ module CrashSafeTree {
 import opened KVTypes
 import TreeDisk
 
+function Last<T>(s:seq<T>) : T  // TODO move to library
+    requires 0<|s|
+{
+    s[|s|-1]
+}
+
 type LBA = TreeDisk.LBA
 type Sector = TreeDisk.Sector
 
@@ -96,37 +102,27 @@ predicate NodeDisownsChild(parent:Sector, childLba:LBA)
 }
 
 datatype Range = Range(loinc:Key, hiexc:Key)
+
 function FULL_RANGE() : Range
 {
     Range(MIN_KEY(), MAX_KEY())
 }
 
+predicate RangeContains(range:Range, key:Key)
+{
+    && KeyLeq(range.loinc, key)
+    && KeyLe(key, range.hiexc)
+}
+
 datatype PathElt = PathElt(
-    node:CRead, // this node
-    idx:int,    // index of Pointer(i+1) in children[] 
-    range:Range // bounds for keys in this node
+    cread:CRead, // this node
+    idx:int,     // index of path[i+1].cread.lba in children[] 
+    range:Range  // bounds for keys at this node
     )    
-
-// True if every Node in path is live (committed) tree data. (The caller cares about the last node.)
-predicate CachedPathRead(k:Constants, s:Variables, path:seq<CRead>)
-{
-    && 0<|path|
-    && path[0].lba == ROOT_LBA()
-    && (forall i :: 0<=i<|path| ==> CachedRead(k, s, path[i]) && path[i].sector.Node?)
-    && (forall i :: 0<=i<|path|-1 ==> !NodeDisownsChild(path[i].sector, path[i+1].lba))
-}
-
-predicate NodeIsLive(k:Constants, s:Variables, node:CRead)
-{
-    exists path :: (
-        && CachedPathRead(k, s, path)
-        && path[-1] == node
-    )
-}
 
 // If all of node's keys are bounded by nodeRange, then
 // the keys in the i'th children of node are bounded by range.
-function RangeBoundsChild(node:Sector, nodeRange:Range, i:int) : (range:Range)
+function RangeBoundForChildIdx(node:Sector, nodeRange:Range, i:int) : (range:Range)
     requires node.Node?
     requires 0<=i<|node.children|
 {
@@ -135,22 +131,32 @@ function RangeBoundsChild(node:Sector, nodeRange:Range, i:int) : (range:Range)
         if i==|node.children|-1 then nodeRange.hiexc else node.pivots[i])
 }
 
-// ranges[i] is a node bound for path[i].
-// path[0] is the root, so ranges[0] is always FULL_RANGE()
-predicate CachedPathReadRanges(k:Constants, s:Variables, path:seq<CRead>, ranges:seq<Range>)
+// True if every Node in path is live (committed) tree data.
+// The caller cares about the last element.
+predicate CachedPathRead(k:Constants, s:Variables, path:seq<PathElt>)
 {
-    && CachedPathRead(k, s, path)
-    && ranges[0] == FULL_RANGE()
-    && (forall i :: 0<=i<|path|-1 ==>
-        ranges[i] == RangeBoundsNode(path[i].sector, ranges[i], IndexOfChild(path[i].sector, path[i+1])))
-    && forall i :: 1<=i<|path| ==> RangeBoundsNode(ranges[i-1], path.sector, ranges[i])
+    && 0<|path|
+    && path[0].cread.lba == ROOT_LBA()
+    && forall i :: 0<=i<|path| ==> (
+        var pElt := path[i];
+        && CachedRead(k, s, pElt.cread)
+        && i<|path|-1 ==> (
+            && pElt.cread.sector.Node?   // TODO factor Node out of Sector
+            && 0 <= pElt.idx < |pElt.cread.sector.children|
+            && pElt.cread.sector.children[i] == TreeDisk.Pointer(path[i+1].cread.lba)
+            )
+        // Ranges next correctly
+        && RangeBoundForChildIdx(pElt.cread.sector, pElt.range, pElt.idx) == path[i+1].range
+        )
+
+    && (forall i :: 0<=i<|path|-1 ==> !NodeDisownsChild(path[i].cread.sector, path[i+1].cread.lba))
 }
 
-predicate NodeIsLiveRange(k:Constants, s:Variables, node:CRead, klo:Key, khi:Key)
+predicate NodeIsLive(k:Constants, s:Variables, node:CRead)
 {
-    exists path :: (
+    exists path:seq<PathElt> :: (
         && CachedPathRead(k, s, path)
-        && path[-1] == node
+        && Last(path).cread == node
     )
 }
 
@@ -212,7 +218,7 @@ predicate KnowPrepared(k:Constants, s:Variables, parentRead:CRead, i:int, childR
     && childRead.sector == ChildNodeForParentIdx(parentRead, i)
 }
 
-function Update(parent:Sector, i:int, child:TreeDisk.Child) : Sector
+function SectorUpdateChild(parent:Sector, i:int, child:TreeDisk.Child) : Sector
     requires parent.Node?
 {
     TreeDisk.Node(parent.parent, parent.pivots,
@@ -222,7 +228,7 @@ function Update(parent:Sector, i:int, child:TreeDisk.Child) : Sector
 predicate CommitGrowAction(k:Constants, s:Variables, s':Variables, parentRead:CRead, i:int, childRead:CRead)
 {
     && KnowPrepared(k, s, parentRead, i, childRead)
-    && WriteThrough(k, s, s', parentRead.lba, Update(parentRead.sector, i,
+    && WriteThrough(k, s, s', parentRead.lba, SectorUpdateChild(parentRead.sector, i,
         TreeDisk.Pointer(childRead.lba)))
 }
 
@@ -233,47 +239,93 @@ predicate ContractNodeAction(k:Constants, s:Variables, s':Variables, parentRead:
     && childRead.sector.Node?
     && childRead.sector.pivots == []    // child has one child, which can take its place in parent.
     && WriteThrough(k, s, s', parentRead.lba,
-        Update(parentRead.sector, i, childRead.sector.children[0]))
+        SectorUpdateChild(parentRead.sector, i, childRead.sector.children[0]))
     // This write causes child to become free-by-unreachable. So child must be in committed warm set.
 }
 
-predicate QueryAction(k:Constants, s:Variables, s':Variables, nodeRead:CRead, datum:Datum)
+// There's a live path leading to node, and it supports range as a bound for node.
+predicate LivePathBoundsChild(k:Constants, s:Variables, node:CRead, idx:int, range:Range)
 {
-    && NodeIsLive(k, s, nodeRead)
-    && 
-    && var child := sector.child[idx]; (
+    exists path : seq<PathElt> :: (
+        && CachedPathRead(k, s, path)
+        && Last(path).cread == node
+        && Last(path).idx == idx
+        && RangeBoundForChildIdx(Last(path).cread.sector, Last(path).range, Last(path).idx) == range
+    )
+}
+
+predicate QueryAction(k:Constants, s:Variables, s':Variables, nodeRead:CRead, idx:int, range:Range, datum:Datum)
+{
+    var childRange := RangeBoundForChildIdx(nodeRead.sector, range, idx);
+    && LivePathBoundsChild(k, s, nodeRead, idx, range)
+    && RangeContains(range, datum.key)
+    && var child := nodeRead.sector.children[idx]; (
         || (child.Value? && child.datum == datum)
         || (child.Value? && child.datum.key != datum.key && datum.value == EmptyValue())
         || (child.Empty? && datum.value == EmptyValue())
         )
 }
 
+// Insert newPivot at idx (shifting old pivot[idx] to the right).
+// Replace child[idx] with newChildren.
+// In practice, |newChildren|=2, and one of its elements is the old child[idx].
+function SectorInsertChild(parent:Sector, idx:int, newPivot:Key, newChildren:seq<TreeDisk.Child>) : Sector
+    requires parent.Node?
+{
+    TreeDisk.Node(parent.parent,
+        parent.pivots[..idx] + [newPivot] + parent.pivots[idx..],
+        parent.children[..idx] + newChildren + parent.children[idx+1..])
+}
+// newDatum.key is absent from the tree; insert it near a neighboring pivot
 predicate InsertAction(k:Constants, s:Variables, s':Variables, newDatum:Datum)
 {
-    var oldDatum := P.children[idx].datum;
-    && KnowPath(datum.key, parent, idx)
-    && WriteThrough(k.disk, s.disk, s'.disk, parent,
-        UpdateInsert(parent, idx, PivotForInsert(oldDatum, newDatum), ChildrenForInsert(oldDatum, newDatum)))
+    exists nodeRead:CRead, range:Range, idx:int :: (
+        // Find a leaf that we can split.
+        var childRange := RangeBoundForChildIdx(nodeRead.sector, range, idx);
+        var extantChild := nodeRead.sector.children[idx];
+        && LivePathBoundsChild(k, s, nodeRead, idx, range)
+        && RangeContains(range, newDatum.key)
+        && !extantChild.Pointer?
+        // This is an insert, not a replace
+        && if extantChild.Empty? || newDatum.key == extantChild.datum.key
+                // Replace an empty or same-key datum in place
+            then WriteThrough(k, s, s', nodeRead.lba,
+                SectorUpdateChild(nodeRead.sector, idx, TreeDisk.Value(newDatum)))
+            else if KeyLe(newDatum.key, extantChild.datum.key)
+                // New datum goes to the left, so we'll split a pivot to the right with the old key
+            then WriteThrough(k, s, s', nodeRead.lba,
+                SectorInsertChild(nodeRead.sector, idx, extantChild.datum.key, [TreeDisk.Value(newDatum), extantChild]))
+                // New datum goes to the right, so we'll split a pivot with the new key
+            else WriteThrough(k, s, s', nodeRead.lba,
+                SectorInsertChild(nodeRead.sector, idx, newDatum.key, [extantChild, TreeDisk.Value(newDatum)]))
+    )
 }
 
-predicate DeleteAction(k:Constants, s:Variables, s':Variables, newDatum:Datum)
+predicate DeleteAction(k:Constants, s:Variables, s':Variables, newDatum:Datum, nodeRead:CRead, idx:int, range:Range)
 {
-    && 1 < |cache[parent].children|
-    && WriteThrough(k.disk, s.disk, s'.disk, parent,
-        UpdateInsert(parent, idx, PivotForInsert(oldDatum, newDatum), ChildrenForInsert(oldDatum, newDatum)))
+    && LivePathBoundsChild(k, s, nodeRead, idx, range)  // don't actually care about range
+    && nodeRead.sector.children[idx] == TreeDisk.Value(newDatum)
+    // Replace child with Empty. TODO background clean up of empty children where feasible.
+    // (Contract cleans up small children.)
+    && WriteThrough(k, s, s', nodeRead.lba,
+        SectorUpdateChild(nodeRead.sector, idx, TreeDisk.Empty))
 }
 
 // Move an unreachable node onto an uncommitted free list
-predicate MoveToFreeListAction(k:Constants, s:Variables, s':Variables, lba:LBA)
+predicate MoveToFreeListAction(k:Constants, s:Variables, s':Variables, lba:LBA, childRead:CRead)
 {
-    && WriteThrough(k.disk, s.disk, s'.disk, ColdFreeList(s.uncommittedFreeListHead))
+    && CachedRead(k, s, childRead)
+    && NodeDisconnected(k, s, childRead)
+    && WriteThrough(k, s, s', lba, TreeDisk.ColdFreeList(s.uncommittedFreeListHead))
     && s'.uncommittedFreeListHead == lba
 }
 
-predicate CommitFreeListAction(k:Constants, s:Variables, s':Variables, lba:LBA)
+predicate CommitFreeListAction(k:Constants, s:Variables, s':Variables, lba:LBA, super:CRead)
 {
-    Write(k.disk, s.disk, s'.disk, SUPERBLOCK_LBA,
-        Superblock(s.uncommittedFreeListHead, super.warm, super.virgin))
+    && super.lba == SUPERBLOCK_LBA()
+    && CachedRead(k, s, super)
+    && WriteThrough(k, s, s', super.lba,
+        TreeDisk.Superblock(s.uncommittedFreeListHead, super.sector.warm, super.sector.virgin))
 }
 
 
