tla-tree/KVTypes.dfy
@@ -1,6 +1,20 @@
 module KVTypes {
 
 type Key(!new,==)
+
+predicate KeyLe(a:Key, b:Key)
+
+predicate KeyLeq(a:Key, b:Key) {
+    KeyLe(a, b) || a==b
+}
+
+function MIN_KEY() : Key
+    ensures forall k :: KeyLeq( MIN_KEY(), k)
+
+function MAX_KEY() : Key
+    ensures forall k :: KeyLeq(k, MAX_KEY())
+
+
 type Value(!new,==)
 datatype Datum = Datum(key:Key, value:Value)
 
